misc/monad_playground.v
@@ -1,0 +1,24 @@
+From Stdlib Require Import Arith.
+From shift_reset.lib Require Import signatures signature_laws.
+From shift_reset.monad Require Import writer transformers.
+From proofs.monad Require Import writer.
+
+Compute (fun R W A => cont_t R (writer_t W identity) A).
+Compute (fun W R A => writer_t W (cont_t R identity) A).
+
+Module NatMonoid <: Monoid.
+  Definition t := nat.
+  Definition empty := O.
+  Definition append := Nat.add.
+End NatMonoid.
+
+Module NatMonoidLaws <: MonoidLaws NatMonoid.
+  Definition append_assoc : forall x y z, x + y + z = x + (y + z).
+  Proof. symmetry. apply Nat.add_assoc. Qed.
+  Definition append_empty_l := Nat.add_0_l.
+  Definition append_empty_r := Nat.add_0_r.
+End NatMonoidLaws.
+
+Module WriterNat := Make NatMonoid.
+Module WriterNatLaws := MakeLaws NatMonoid NatMonoidLaws WriterNat.
+Print WriterNatLaws.
