misc/test.v
@@ -1,4 +1,0 @@
-From shift_reset.lib Require Import monad_transformer.
-
-Compute (fun R W A => cont_t R (writer_t W identity) A).
-Compute (fun W R A => writer_t W (cont_t R identity) A).
