proofs/monad/writer.v
@@ -1,0 +1,63 @@
+From shift_reset.lib Require Import signatures signature_laws.
+From shift_reset.monad Require Import writer.
+
+Lemma map_id {W A} (m : writer W A) :
+  map (fun x => x) m = m.
+Proof.
+  cbv.
+  destruct m as [m].
+  destruct m as [x w].
+  reflexivity.
+Qed.
+
+Lemma map_comp {W A B C} (f : B -> C) (g : A -> B) (m : writer W A) :
+  map f (map g m) = map (fun x => f (g x)) m.
+Proof.
+  cbv. f_equal.
+  destruct m as [m].
+  destruct m as [x w].
+  reflexivity.
+Qed.
+
+Module Type MakeSig (M : Monoid).
+  Include Make M.
+End MakeSig.
+
+Module MakeLaws (W : Monoid) (WLaws : MonoidLaws W) (MSig : MakeSig W).
+  Import WLaws.
+  Import MSig.
+
+  Lemma pure_bind {A B} (x : A) (f : A -> writer W.t B) :
+    bind (pure x) f = f x.
+  Proof.
+    cbv.
+    destruct (f x) as [m].
+    destruct m as [y w].
+    rewrite -> append_empty_l.
+    reflexivity.
+  Qed.
+
+  Lemma bind_pure {A} (m : writer W.t A) :
+    bind m pure = m.
+  Proof.
+    cbv.
+    destruct m as [m].
+    destruct m as [x w].
+    rewrite -> append_empty_r.
+    reflexivity.
+  Qed.
+
+  Lemma bind_assoc {A B C} (m : writer W.t A) (f : A -> writer W.t B) (g : B -> writer W.t C) :
+    bind (bind m f) g = bind m (fun x => bind (f x) g).
+  Proof.
+    cbv. f_equal.
+    destruct m as [m].
+    destruct m as [x w].
+    destruct (f x) as [m].
+    destruct m as [y w'].
+    destruct (g y) as [m].
+    destruct m as [z w''].
+    rewrite -> append_assoc.
+    reflexivity.
+  Qed.
+End MakeLaws.
