shift-reset/lib/gmap.v
@@ -9,7 +9,8 @@ Module Type IsoPositiveType.
   Axiom encode_decode : forall (x : positive), encode (decode x) = x.
 End IsoPositiveType.
 
-Record gmap (K A : Type) := GMap { gmap_car : pmap.pmap A }.
+Record gmap (K A : Type) := GMap { gmap_car : pmap.t A }.
+Definition t : Type -> Type -> Type := gmap.
 
 Arguments GMap {K A} _.
 Arguments gmap_car {K A} _.
@@ -23,24 +24,21 @@ Definition filter_map {K A B} (f : A -> option B) (mt : gmap K A) : gmap K B :=
   GMap (pmap.filter_map f (gmap_car mt)).
 
 Module Make (K : IsoPositiveType).
-  Definition key : Type := K.t.
-  Definition t : Type -> Type := gmap key.
-
-  Definition find {A} (k : key) (mt : gmap key A) : option A :=
+  Definition find {A} (k : K.t) (mt : gmap K.t A) : option A :=
     pmap.find (K.encode k) (gmap_car mt).
 
-  Definition member {A} (k : key) (mt : gmap key A) : bool :=
+  Definition member {A} (k : K.t) (mt : gmap K.t A) : bool :=
     pmap.member (K.encode k) (gmap_car mt).
 
-  Definition singleton {A} (k : key) (x : A) : gmap key A :=
+  Definition singleton {A} (k : K.t) (x : A) : gmap K.t A :=
     GMap (pmap.singleton (K.encode k) x).
 
-  Definition add {A} (k : key) (x : A) (mt : gmap key A) : gmap key A :=
+  Definition add {A} (k : K.t) (x : A) (mt : gmap K.t A) : gmap K.t A :=
     GMap (pmap.add (K.encode k) x (gmap_car mt)).
 
-  Definition remove {A} (k : key) (mt : gmap key A) : gmap key A :=
+  Definition remove {A} (k : K.t) (mt : gmap K.t A) : gmap K.t A :=
     GMap (pmap.remove (K.encode k) (gmap_car mt)).
 
-  Definition update {A} (f : option A -> option A) (k : key) (mt : gmap key A) : gmap key A :=
-    GMap (pmap.update f (K.encode k) (gmap_car mt)).
+  Definition update {A} (k : K.t) (f : option A -> option A) (mt : gmap K.t A) : gmap K.t A :=
+    GMap (pmap.update (K.encode k) f (gmap_car mt)).
 End Make.
